CollapsingTowers/TwoLevelRec/SyntacticSoundness/Preservation.lean
@@ -3,9 +3,9 @@ import CollapsingTowers.TwoLevelRec.SyntacticSoundness.PresvHead
 theorem preservation.strengthened :
   ∀ Γ e₀ e₁ τ φ₀,
     step_lvl Γ.length e₀ e₁ →
-    typing Γ 𝟚 e₀ τ φ₀ →
+    typing_reification Γ e₀ τ φ₀ →
     ∃ φ₁,
-      typing Γ 𝟚 e₁ τ φ₁ ∧
+      typing_reification Γ e₁ τ φ₁ ∧
       φ₁ ≤ φ₀ :=
   by
   intro Γ e₀ e₁ τ φ₀
@@ -13,9 +13,6 @@ theorem preservation.strengthened :
   intro Hstep Hτ
   cases Hstep
   case pure HM Hlc Hhead =>
-    induction HM generalizing Γ τ φ₀
-    case hole => apply preservation.head _ _ _ _ _ Hhead Hτ
-    case cons𝔹 => admit
-    case consℝ => admit
+    admit
   case reflect P E e HP HE Hlc =>
     admit
