CollapsingTowers/TwoLevelRec/SyntacticSoundness/PresvMaping.lean
@@ -3,8 +3,8 @@ import CollapsingTowers.TwoLevelRec.SyntacticTyping.Weakening
 lemma preservation.maping.strengthened :
   ∀ Γ Δ Φ v e τ𝕒 τ𝕓 τ𝕔 𝕊𝕒 𝕊𝕓 φ,
     typing Γ 𝕊𝕓 e τ𝕓 φ →
-    Γ = Δ ++ (τ𝕔, 𝟚) :: Φ →
-    typing (Δ ++ (τ𝕒, 𝕊𝕒) :: Φ) 𝟚 v τ𝕔 ⊥ →
+    Γ = Δ ++ (τ𝕔, 𝟙) :: Φ →
+    typing (Δ ++ (τ𝕒, 𝕊𝕒) :: Φ) 𝟙 v τ𝕔 ⊥ →
     typing (Δ ++ (τ𝕒, 𝕊𝕒) :: Φ) 𝕊𝕓 (subst Φ.length v e) τ𝕓 φ :=
   by
   intros Γ Δ Φ v e τ𝕒 τ𝕓 τ𝕔 𝕊𝕒 𝕊𝕓 φ Hτe HEqΓ Hτv
@@ -13,13 +13,13 @@ lemma preservation.maping.strengthened :
     @typing.rec
       (fun Γ 𝕊 e τ𝕓 φ (H : typing Γ 𝕊 e τ𝕓 φ) =>
         ∀ Δ,
-          Γ = Δ ++ (τ𝕔, 𝟚) :: Φ →
-          typing (Δ ++ (τ𝕒, 𝕊𝕒) :: Φ) 𝟚 v τ𝕔 ⊥ →
+          Γ = Δ ++ (τ𝕔, 𝟙) :: Φ →
+          typing (Δ ++ (τ𝕒, 𝕊𝕒) :: Φ) 𝟙 v τ𝕔 ⊥ →
           typing (Δ ++ (τ𝕒, 𝕊𝕒) :: Φ) 𝕊 (subst Φ.length v e) τ𝕓 φ)
       (fun Γ e τ𝕓 φ (H : typing_reification Γ e τ𝕓 φ) =>
         ∀ Δ,
-          Γ = Δ ++ (τ𝕔, 𝟚) :: Φ →
-          typing (Δ ++ (τ𝕒, 𝕊𝕒) :: Φ) 𝟚 v τ𝕔 ⊥ →
+          Γ = Δ ++ (τ𝕔, 𝟙) :: Φ →
+          typing (Δ ++ (τ𝕒, 𝕊𝕒) :: Φ) 𝟙 v τ𝕔 ⊥ →
           typing_reification (Δ ++ (τ𝕒, 𝕊𝕒) :: Φ) (subst Φ.length v e) τ𝕓 φ)
   <;> intros
   case fvar 𝕊 x _ HBinds Hwbt Δ HEqΓ Hτv =>
@@ -29,11 +29,11 @@ lemma preservation.maping.strengthened :
       rw [compare_lt_iff_lt] at Hx
       simp [if_neg (Nat.ne_of_lt Hx)]
       apply typing.fvar
-      . have HEq : x = x - ((τ𝕔, 𝟚) :: Φ).length + ((τ𝕒, 𝕊𝕒) :: Φ).length := by simp; omega
+      . have HEq : x = x - ((τ𝕔, 𝟙) :: Φ).length + ((τ𝕒, 𝕊𝕒) :: Φ).length := by simp; omega
         rw [HEq]
         apply binds.extendr
         apply binds.shrinkr
-        have HEq : x - ((τ𝕔, 𝟚) :: Φ).length + ((τ𝕔, 𝟚) :: Φ).length = x := by simp; omega
+        have HEq : x - ((τ𝕔, 𝟙) :: Φ).length + ((τ𝕔, 𝟙) :: Φ).length = x := by simp; omega
         rw [HEq]
         apply HBinds
       . apply Hwbt
@@ -60,11 +60,11 @@ lemma preservation.maping.strengthened :
       rw [compare_lt_iff_lt] at Hx
       simp [if_neg (Nat.ne_of_lt Hx)]
       apply typing.code_fragment
-      . have HEq : x = x - ((τ𝕔, 𝟚) :: Φ).length + ((τ𝕒, 𝕊𝕒) :: Φ).length := by simp; omega
+      . have HEq : x = x - ((τ𝕔, 𝟙) :: Φ).length + ((τ𝕒, 𝕊𝕒) :: Φ).length := by simp; omega
         rw [HEq]
         apply binds.extendr
         apply binds.shrinkr
-        have HEq : x - ((τ𝕔, 𝟚) :: Φ).length + ((τ𝕔, 𝟚) :: Φ).length = x := by simp; omega
+        have HEq : x - ((τ𝕔, 𝟙) :: Φ).length + ((τ𝕔, 𝟙) :: Φ).length = x := by simp; omega
         rw [HEq]
         apply HBinds
       . apply Hwbt
@@ -86,7 +86,7 @@ lemma preservation.maping.strengthened :
     simp [HEqΓ] at Hclosed
     rw [HEqΓ] at IH
     apply typing.lam
-    . have HEq : (Δ ++ (τ𝕒, 𝕊𝕒) :: Φ).length = (Δ ++ (τ𝕔, 𝟚) :: Φ).length := by simp
+    . have HEq : (Δ ++ (τ𝕒, 𝕊𝕒) :: Φ).length = (Δ ++ (τ𝕔, 𝟙) :: Φ).length := by simp
       rw [HEq, ← comm.subst_opening]
       apply IH (_ :: Δ) rfl
       apply typing.weakening.singleton _ _ _ _ _ _ _ Hτv
@@ -100,7 +100,7 @@ lemma preservation.maping.strengthened :
     simp [HEqΓ] at Hclosed
     rw [HEqΓ] at IH
     apply typing.lam𝕔
-    . have HEq : (Δ ++ (τ𝕒, 𝕊𝕒) :: Φ).length = (Δ ++ (τ𝕔, 𝟚) :: Φ).length := by simp
+    . have HEq : (Δ ++ (τ𝕒, 𝕊𝕒) :: Φ).length = (Δ ++ (τ𝕔, 𝟙) :: Φ).length := by simp
       rw [HEq, ← comm.subst_opening]
       apply IH (_ :: Δ) rfl
       apply typing.weakening.singleton _ _ _ _ _ _ _ Hτv
@@ -144,7 +144,7 @@ lemma preservation.maping.strengthened :
     rw [HEqΓ] at IHe
     apply typing.lets
     . apply IHb; apply HEqΓ; apply Hτv
-    . have HEq : (Δ ++ (τ𝕒, 𝕊𝕒) :: Φ).length = (Δ ++ (τ𝕔, 𝟚) :: Φ).length := by simp
+    . have HEq : (Δ ++ (τ𝕒, 𝕊𝕒) :: Φ).length = (Δ ++ (τ𝕔, 𝟙) :: Φ).length := by simp
       rw [HEq, ← comm.subst_opening]
       apply IHe (_ :: Δ) rfl
       apply typing.weakening.singleton _ _ _ _ _ _ _ Hτv
@@ -159,7 +159,7 @@ lemma preservation.maping.strengthened :
     rw [HEqΓ] at IHe
     apply typing.lets𝕔
     . apply IHb; apply HEqΓ; apply Hτv
-    . have HEq : (Δ ++ (τ𝕒, 𝕊𝕒) :: Φ).length = (Δ ++ (τ𝕔, 𝟚) :: Φ).length := by simp
+    . have HEq : (Δ ++ (τ𝕒, 𝕊𝕒) :: Φ).length = (Δ ++ (τ𝕔, 𝟙) :: Φ).length := by simp
       rw [HEq, ← comm.subst_opening]
       apply IHe (_ :: Δ) rfl
       apply typing.weakening.singleton _ _ _ _ _ _ _ Hτv
@@ -202,9 +202,9 @@ lemma preservation.maping.strengthened :
 
 theorem preservation.maping :
   ∀ Γ v e τ𝕒 τ𝕓 τ𝕔 𝕊 φ,
-    typing ((τ𝕔, 𝟚) :: Γ) 𝟚 e τ𝕓 φ →
-    typing ((τ𝕒, 𝕊) :: Γ) 𝟚 v τ𝕔 ⊥ →
-    typing ((τ𝕒, 𝕊) :: Γ) 𝟚 (subst Γ.length v e) τ𝕓 φ :=
+    typing ((τ𝕔, 𝟙) :: Γ) 𝟙 e τ𝕓 φ →
+    typing ((τ𝕒, 𝕊) :: Γ) 𝟙 v τ𝕔 ⊥ →
+    typing ((τ𝕒, 𝕊) :: Γ) 𝟙 (subst Γ.length v e) τ𝕓 φ :=
   by
   intros Γ v e τ𝕒 τ𝕓 τ𝕔 𝕊 φ Hτe Hτv
-  apply preservation.maping.strengthened _ [] _ _ _ _ _ _ _ _ _ Hτe rfl Hτv
+  apply preservation.maping.strengthened _ ⦰ _ _ _ _ _ _ _ _ _ Hτe rfl Hτv
